\subsection{State-space representation}
In the following representation, all the $y$ in the diagram have been replaced by $d$.\par
Input vector $U$ and state vector $X$ are given by :
$$
U = \begin{pmatrix}
    F_1 \\
    u
\end{pmatrix}
\hspace{3cm}
X = \begin{pmatrix}
    d_1 \\
    \dot d_1 \\
    d_2 \\ 
    \dot d_2 \\
\end{pmatrix}
$$

% Inputs
\subsubsection{Inputs}
\begin{itemize}
    \item $F_1(t)$, the force of the wind (uncontrollable).
    \item $u(t)$, the force applied on the mass damper (controllable).
\end{itemize}
Our sensor is a measurement of the horizontal position of the top of the building relatively to the vertical position $d_1 = 0$.\par
Our actuator provides a force on the mass of the dampener, sets it in motion.

% Outputs
\subsubsection{Outputs}
$y = d_1(t)$ the relative position of the building with respect to the vertical position.

% States
\subsubsection{States}
\begin{itemize}
    \item $x_1 = d_1$, as described above.
    \item $x_2 = \dot d_1$, the speed of the building.
    \item $x_3 = d_2$, the relative displacement of the mass damper.
    \item $x_4 = \dot d_2$, the speed of the mass damper.
\end{itemize}

% Output law
\subsubsection{Output law}
The output is one of the states : $y = x_1$.

% Input law
\subsubsection{Input law}
The input law is given by \cite{science_direct} :
$$
\begin{cases}
    m_{1}\ddot{d}_{1} + c_{1}\dot{d}_{1} + k_{1}d_{1} = c_{2}\dot{z} + k_{2}z + F_{1}(t) - u(t)\\
    m_{2}\ddot{z} + c_{2}\dot{z} + k_{2}z = -m_{2}\ddot{d}_{1} + u(t)
\end{cases}
$$
with $z = d_2 - d_1$.\par
The system is \textbf{linear}. We can easily derive the ABCD matrices.
$$
A = \begin{pmatrix}
    0 & 1 & 0 & 0 \\
    \frac{-k_1-k_2}{m_1} & \frac{-c_2-c_1}{m_1} & \frac{k_2}{m_1} & \frac{c_2}{m_1} \\
    0 & 0 & 0 & 1 \\ 
    \frac{k_2}{m_2} & \frac{c_2}{m_2} & \frac{-k_2}{m_2} & \frac{-c_2}{m_2}\\
\end{pmatrix}
\quad
B = \begin{pmatrix}
    0 & 0\\
    \frac{1}{m_1} & -\frac{1}{m_1}\\
    0 & 0\\
    0 & \frac{1}{m_2}\\
\end{pmatrix}
$$
$$
C = \begin{pmatrix}
    1 & 0 & 0 & 0\\
\end{pmatrix}
\quad
D = \begin{pmatrix}
    0 & 0\\
\end{pmatrix}
$$
